safechecker/theories/PCUICSafeReduce.v
@@ -56,7 +56,7 @@ Qed.
 *)
 Section Measure.
 
-  Context {cf : checker_flags}.
+  Context {cf : checker_flags} {cu : check_univs_tc}.
 
   Context (flags : RedFlags.t).
   Context (Σ : global_env_ext).
@@ -70,12 +70,11 @@ Section Measure.
 
   Lemma cored_welltyped :
     forall {Γ u v},
-      ∥ wf Σ ∥ -> welltyped Σ Γ u ->
+      wf Σ -> welltyped Σ Γ u ->
       cored Σ Γ v u ->
       welltyped Σ Γ v.
   Proof.
     intros Γ u v HΣ h r.
-    destruct HΣ as [wΣ].
     revert h. induction r ; intros h.
     - destruct h as [A HA]. exists A.
       eapply subject_reduction1 ; eassumption.
@@ -86,11 +85,11 @@ Section Measure.
 
   Lemma red_welltyped :
     forall {Γ u v},
-      ∥ wf Σ ∥ -> welltyped Σ Γ u ->
-      ∥ red (fst Σ) Γ u v ∥ ->
+      wf Σ -> welltyped Σ Γ u ->
+      red (fst Σ) Γ u v ->
       welltyped Σ Γ v.
   Proof.
-    intros hΣ Γ u v h [r]. apply red_cored_or_eq in r.
+    intros hΣ Γ u v h r. apply red_cored_or_eq in r.
     destruct r as [r|[]]; [|assumption].
     eapply cored_welltyped ; eauto.
   Qed.
@@ -211,13 +210,14 @@ Opaque Acc_intro_generator.
 
 Section Reduce.
 
-  Context {cf : checker_flags}.
+  Context {cf : checker_flags} {cu : check_univs_tc}.
 
   Context (flags : RedFlags.t).
 
   Context (Σ : global_env_ext).
   Context (heΣ : ∥ wf_ext Σ ∥).
-  Let hΣ := map_squash (wf_ext_wf _) heΣ.
+
+  Local Definition hΣ : ∥ wf Σ ∥ := map_squash (wf_ext_wf Σ) heΣ.
 
   Existing Instance Req_refl.
 
@@ -477,11 +477,12 @@ Section Reduce.
     symmetry. assumption.
   Qed.
   Next Obligation.
+    pose proof (hΣ := hΣ).
+    sq.
     pose proof (welltyped_context _ hΣ _ _ h) as hc.
     simpl in hc.
     (* Should be a lemma! *)
-    destruct hΣ as [wΣ].
-    clear - eq hc wΣ.
+    clear - eq hc hΣ.
     revert c hc eq.
     generalize (Γ ,,, stack_context π) as Δ. clear Γ π.
     intro Γ.
@@ -728,24 +729,27 @@ Section Reduce.
   Qed.
   Next Obligation.
     clear eq.
-    destruct hΣ.
+    pose proof (hΣ := hΣ).
+    sq.
     unfold Pr in p0. cbn in p0.
     pose proof p0 as hh.
     rewrite <- prf' in hh. cbn in hh. subst.
     apply eq_sym, decompose_stack_eq in prf'; subst.
     apply Req_red in r; cbn in r.
+    sq.
     rewrite zipc_appstack in r.
     cbn in r.
-    pose proof r as [r'].
-    eapply red_welltyped in r; eauto.
-    zip fold in r.
-    apply welltyped_context in r as (?&typ); auto; cbn in *.
+    pose proof r as r'.
+    eapply red_welltyped in r' ; tea.
+    zip fold in r'.
+    apply welltyped_context in r' as (?&typ); auto; cbn in *.
     apply PCUICInductiveInversion.invert_Case_Construct in typ as H; auto.
+    2: now sq.
     destruct H as (?&?&nth&?); subst.
     rewrite nth in eqbr; noconf eqbr.
     constructor.
     eapply cored_red_cored; cycle 1.
-    - zip fold in r'; exact r'.
+    - zip fold in r; exact r.
     - constructor.
       eapply red1_context.
       eapply red_iota; eauto.
@@ -753,33 +757,37 @@ Section Reduce.
   Qed.
   Next Obligation.
     clear eq.
-    destruct hΣ.
+    pose proof (hΣ := hΣ).
+    sq.
     unfold Pr in p0. cbn in p0.
     pose proof p0 as hh.
     rewrite <- prf' in hh. cbn in hh. subst.
     apply eq_sym, decompose_stack_eq in prf'; subst.
     apply Req_red in r; cbn in r.
+    sq.
     rewrite zipc_appstack in r.
     cbn in r.
-    pose proof r as [r'].
+    pose proof r as r'.
     eapply red_welltyped in r; eauto.
     zip fold in r.
     apply welltyped_context in r as (?&typ); auto; cbn in *.
     apply PCUICInductiveInversion.invert_Case_Construct in typ as H; auto.
+    2: now sq.
     destruct H as (?&?&nth&?); subst.
     rewrite nth in bot; congruence.
   Qed.
   Next Obligation.
     clear eq.
-    destruct hΣ.
+    sq.
     unfold Pr in p0. cbn in p0.
     pose proof p0 as hh.
     rewrite <- prf' in hh. cbn in hh. subst.
     apply eq_sym, decompose_stack_eq in prf'; subst.
     apply Req_red in r; cbn in r.
+    sq.
     rewrite zipc_appstack in r.
     cbn in r.
-    pose proof r as [r'].
+    pose proof r as r'.
     eapply red_welltyped in r; eauto.
     zip fold in r.
     apply welltyped_context in r as (?&typ); auto; cbn in *.
@@ -792,13 +800,14 @@ Section Reduce.
   Qed.
   Next Obligation.
     clear eq.
-    destruct hΣ.
+    sq.
     unfold Pr in p0. cbn in p0.
     pose proof p0 as hh.
     rewrite <- prf' in hh. cbn in hh. subst.
     apply eq_sym, decompose_stack_eq in prf'; subst.
     apply Req_red in r; cbn in r.
-    pose proof r as [r'].
+    sq.
+    pose proof r as r'.
     eapply red_welltyped in r; eauto.
     zip fold in r.
     apply welltyped_context in r as (?&typ); auto; cbn in *.
@@ -837,10 +846,12 @@ Section Reduce.
     constructor.
   Qed.
   Next Obligation.
+    pose proof (hΣ := hΣ).
+    sq.
     left.
     apply Req_red in r as hr.
+    sq.
     pose proof (red_welltyped _ hΣ h hr) as hh.
-    destruct hr as [hr].
     eapply cored_red_cored ; try eassumption.
     unfold Pr in p. simpl in p. pose proof p as p'.
     rewrite <- prf' in p'. simpl in p'. subst.
@@ -854,12 +865,15 @@ Section Reduce.
     subst. constructor. eauto.
   Qed.
   Next Obligation.
+    pose proof (hΣ := hΣ).
+    sq.
     unfold Pr in p. simpl in p.
     pose proof p as p'.
     rewrite <- prf' in p'. simpl in p'. subst.
     symmetry in prf'. apply decompose_stack_eq in prf' as ?.
     subst.
     apply Req_red in r as hr.
+    sq.
     pose proof (red_welltyped _ hΣ h hr) as hh.
     cbn in hh. rewrite zipc_appstack in hh. cbn in hh.
     zip fold in hh.
@@ -894,7 +908,8 @@ Section Reduce.
         constructor. eapply red_cofix_proj. eauto. 
   Qed.
   Next Obligation.
-    destruct hΣ as [wΣ].
+    pose proof (hΣ := hΣ).
+    sq.
     unfold Pr in p. simpl in p.
     pose proof p as p'.
     rewrite <- prf' in p'. simpl in p'. subst.
@@ -906,7 +921,6 @@ Section Reduce.
       - clear eq. dependent destruction r.
         + apply cored_red in H. destruct H as [r].
           eapply red_welltyped ; eauto.
-          constructor.
           symmetry in prf'. apply decompose_stack_eq in prf'. subst.
           cbn in r. rewrite zipc_appstack in r. cbn in r.
           assumption.
@@ -918,7 +932,8 @@ Section Reduce.
     replace (zip (tProj (i, pars, narg) (mkApps (tCoFix mfix idx) args), π))
       with (zip (tCoFix mfix idx, appstack args (Proj (i, pars, narg) :: π)))
       in h'.
-    - destruct hΣ.
+    - pose proof (hΣ := hΣ).
+      sq.
       apply welltyped_context in h' ; auto. simpl in h'.
       destruct h' as [T h'].
       apply inversion_CoFix in h' ; auto.
@@ -961,6 +976,8 @@ Section Reduce.
     forall x y : term × stack, welltyped Σ Γ (zip x) -> R Σ Γ y x -> welltyped Σ Γ (zip y).
   Proof.
     intros x y H HR.
+    pose proof (hΣ := hΣ).
+    sq.
     depelim HR.
     - eapply cored_welltyped; eauto.
     - simpl in H1. revert H1; intros [= H2 _].
@@ -989,20 +1006,20 @@ Section Reduce.
           inversion H1. subst. inversion H2. subst. clear H1 H2.
           intros. cbn. rewrite H3. assumption.
   Defined.
-(*   Next Obligation.
-    destruct hΣ.
-    eapply R_Acc. all: assumption.
-  Defined.
- *)
-  (* Replace the last obligation by the following to run inside Coq. *)
   Next Obligation.
+    sq.
+    now eapply R_Acc.
+    Unshelve.
+  Defined.
+  (* Replace the last obligation by the following to run inside Coq. *)
+  (* Next Obligation.
     revert h. generalize (t, π).
     refine (Acc_intro_generator
               (R:=fun x y => R Σ Γ x y)
               (P:=fun x => welltyped Σ Γ (zip x)) (fun x y Px Hy => _) 1000 _).
     - simpl in *. eapply welltyped_R_pres; eauto.
     - destruct heΣ. intros; eapply R_Acc; eassumption.
-  Defined.
+  Defined. *)
 
   Definition reduce_stack Γ t π h :=
     let '(exist ts _) := reduce_stack_full Γ t π h in ts.
@@ -1361,6 +1378,7 @@ Section Reduce.
       destruct hd; try easy.
       destruct p as ((?&?)&?).
       eapply PCUICInductiveInversion.invert_Proj_Construct in typ' as (->&->&?); auto.
+      2: exact hΣ.
       congruence.
     - unfold isCoFix_app.
       now rewrite decompose_app_mkApps; destruct hd.
@@ -1406,6 +1424,7 @@ Section Reduce.
         destruct l.
         * simpl. eauto with pcuic.
         * exfalso.
+          
           destruct hΣ.
           cbn in h. zip fold in h. apply welltyped_context in h; auto.
           simpl in h. rewrite stack_context_appstack in h.
@@ -1426,7 +1445,9 @@ Section Reduce.
           apply inversion_App in h as (?&?&?&?&?); auto.
           apply inversion_Prod in t0 as (?&?&?&?&?); auto.
           eapply PCUICConversion.equality_Sort_Prod_inv; eauto.
-      + exfalso.
+      + pose proof hΣ.
+        sq.
+        exfalso.
         eapply welltyped_context in h as [s Hs]; tas.
         now eapply inversion_Prim in Hs.
     - unfold zipp. case_eq (decompose_stack π). intros l ρ e.
@@ -1519,6 +1540,7 @@ Section Reduce.
           destruct (reduce x y z)
       end.
       noconf eq3; cbn in *.
+      pose proof hΣ as [hΣ].
       clear -hΣ eq4 ht eq2 eq1 h prf haux.
       destruct prf as (r&stacks&?).
       unfold Pr in stacks.
@@ -1535,8 +1557,7 @@ Section Reduce.
       rewrite zipc_appstack in h.
       apply Req_red in r as [r].
       cbn in *.
-      eapply red_welltyped in h; eauto using sq.
-      clear r.
+      eapply red_welltyped in h; eauto.
       rewrite zipc_appstack in h.
       cbn in h.
       rewrite tApp_mkApps in h.
@@ -1559,7 +1580,7 @@ Section Reduce.
       rewrite app_nil_r in *.
       rewrite <- app_assoc in *.
       cbn in *.
-      destruct hΣ, haux.
+      destruct haux.
       symmetry in eq1.
       constructor.
       constructor.
@@ -1579,6 +1600,7 @@ Section Reduce.
           destruct (reduce x y z)
       end.
       noconf eq; cbn in *.
+      pose proof hΣ as [hΣ].
       clear -hΣ ht prf' h prf haux.
       destruct prf as (r&stacks&?).
       unfold Pr in stacks.
@@ -1609,7 +1631,7 @@ Section Reduce.
         try rewrite stack_context_appstack in H;
         cbn in * ).
       rewrite app_nil_r in *.
-      destruct hΣ, haux.
+      destruct haux.
       constructor.
       apply whnf_mkApps, whne_case.
       eapply whnf_case_arg_whne; eauto.
@@ -1639,7 +1661,8 @@ Section Reduce.
           destruct (reduce x y z)
       end.
       noconf eq; cbn in *.
-      clear -hΣ ht prf' h prf haux.
+      pose proof hΣ as [hΣ].
+      clear -hΣ heΣ ht prf' h prf haux.
       destruct prf as (r&stacks&?).
       unfold Pr in stacks.
       cbn in *.
@@ -1669,7 +1692,7 @@ Section Reduce.
         try rewrite stack_context_appstack in H;
         cbn in * ).
       rewrite app_nil_r in *.
-      destruct hΣ, haux.
+      destruct haux.
       constructor. apply whnf_mkApps, whne_proj.
       eapply whnf_proj_arg_whne; eauto.
       destruct H as (noapp&_).
@@ -1718,7 +1741,7 @@ Section Reduce.
 End Reduce.
 
 Section ReduceFns.
-  Context {cf : checker_flags} {Σ : global_env_ext} (HΣ : ∥ wf_ext Σ ∥).
+  Context {cf : checker_flags} {cu : check_univs_tc} {Σ : global_env_ext} (HΣ : ∥ wf_ext Σ ∥).
 
   (* We get stack overflow on Qed after Equations definitions when this is transparent *)
   Opaque reduce_stack_full.
@@ -1728,8 +1751,7 @@ Section ReduceFns.
   Theorem hnf_sound {Γ t h} : ∥ Σ ;;; Γ ⊢ t ⇝ hnf Γ t h ∥.
   Proof.
     unfold hnf.
-    destruct HΣ.
-    destruct (reduce_term_sound RedFlags.default _ (sq w) _ _ h).
+    destruct (reduce_term_sound RedFlags.default _ HΣ _ _ h).
     sq. eapply into_closed_red; fvs.
   Defined.
   
@@ -1979,7 +2001,7 @@ Section ReduceFns.
   Qed.
   
   Local Instance wellfounded : WellFounded (@hnf_subterm_rel _ Σ) :=
-    @wf_hnf_subterm _ _ HΣ.
+    @wf_hnf_subterm _ _ _ HΣ.
   
   Equations? (noeqns) reduce_to_arity (Γ : context) (T : term) (wt : welltyped Σ Γ T)
     : (conv_arity Γ T) + {~Is_conv_to_Arity Σ Γ T}
